6章：適当にパーサーつけた。修正の余地あり

untype_lambda/ocaml/chap6/main.ml
@@ -1,0 +1,40 @@
+open Arith
+
+let write t =
+  let parse = Parser.toplevel Lexer.main t in
+  let result = Print.eval parse in
+  print_string ((Print.eval_string parse) ^ " -> "); print_string (Print.eval_string result); print_newline()
+
+
+let rec get () =
+  let getin () =
+  let lexbuf = Lexing.from_channel stdin in
+    write lexbuf; get ()
+  in
+  try getin ()
+  with
+      Lexer.Error m  -> print_string m; print_newline(); get() 
+    | Parser.Error -> print_string "Parser Error"; print_newline(); get()
+
+
+let readfile () = 
+      let file = Sys.argv.(1) in
+      let oc   = open_in file in
+      let rec loop () = 
+        let rec ww () =
+            let line = input_line oc in
+            let lexbuf = Lexing.from_string line in 
+            write lexbuf; ww ()
+          in
+          try ww ()
+          with
+            End_of_file     -> close_in oc
+          | Lexer.Error mes -> print_string mes; print_newline(); loop ()
+          | Parser.Error    -> print_string "Parser Error"; print_newline(); loop () in
+      loop ()
+
+let () =
+  match (Array.length Sys.argv) with
+    1 -> get ()
+  | _ -> readfile ()
+
