untype_lambda/ocaml/chap6/src/eval.ml
@@ -1,0 +1,100 @@
+
+type bool =
+| True
+| False
+
+type nat =
+| O
+| S of nat
+
+(** val add : nat -> nat -> nat **)
+
+let rec add n m =
+  match n with
+  | O -> m
+  | S p -> S (add p m)
+
+(** val sub : nat -> nat -> nat **)
+
+let rec sub n m =
+  match n with
+  | O -> n
+  | S k -> (match m with
+            | O -> n
+            | S l -> sub k l)
+
+(** val eqb : nat -> nat -> bool **)
+
+let rec eqb n m =
+  match n with
+  | O -> (match m with
+          | O -> True
+          | S _ -> False)
+  | S n' -> (match m with
+             | O -> False
+             | S m' -> eqb n' m')
+
+(** val leb : nat -> nat -> bool **)
+
+let rec leb n m =
+  match n with
+  | O -> True
+  | S n' -> (match m with
+             | O -> False
+             | S m' -> leb n' m')
+
+type term =
+| Var of nat
+| Abs of term
+| App of term * term
+
+(** val shift : nat -> nat -> term -> term **)
+
+let rec shift d c = function
+| Var k -> (match leb c k with
+            | True -> (match d with
+                       | O -> Var (sub k (S O))
+                       | S _ -> Var (add k d))
+            | False -> Var k)
+| Abs t1 -> Abs (shift d (add c (S O)) t1)
+| App (t1, t2) -> App ((shift d c t1), (shift d c t2))
+
+(** val up : nat -> term -> term **)
+
+let up n t =
+  shift n O t
+
+(** val subst : nat -> term -> term -> term **)
+
+let rec subst j s = function
+| Var k -> (match eqb j k with
+            | True -> s
+            | False -> Var k)
+| Abs t1 -> Abs (subst (add j (S O)) (up (S O) s) t1)
+| App (t1, t2) -> App ((subst j s t1), (subst j s t2))
+
+(** val vb : term -> bool **)
+
+let vb = function
+| Abs _ -> True
+| _ -> False
+
+type optiont =
+| Some of term
+| None
+
+(** val step : term -> optiont **)
+
+let rec step = function
+| App (t1, t2) ->
+  (match t1 with
+   | Abs t3 ->
+     (match vb t2 with
+      | True -> Some (up O (subst O (up (S O) t2) t3))
+      | False -> (match step t2 with
+                  | Some t2' -> Some (App (t1, t2'))
+                  | None -> None))
+   | _ -> (match step t1 with
+           | Some t1' -> Some (App (t1', t2))
+           | None -> None))
+| _ -> None
