untype_lambda/ocaml/chap6/src/eval.mli
@@ -1,0 +1,35 @@
+
+type bool =
+| True
+| False
+
+type nat =
+| O
+| S of nat
+
+val add : nat -> nat -> nat
+
+val sub : nat -> nat -> nat
+
+val eqb : nat -> nat -> bool
+
+val leb : nat -> nat -> bool
+
+type term =
+| Var of nat
+| Abs of term
+| App of term * term
+
+val shift : nat -> nat -> term -> term
+
+val up : nat -> term -> term
+
+val subst : nat -> term -> term -> term
+
+val vb : term -> bool
+
+type optiont =
+| Some of term
+| None
+
+val step : term -> optiont
