untype_lambda/ocaml/chap6/src/lexer.mll
@@ -1,0 +1,16 @@
+{
+  exception Error of string
+}
+
+rule main = parse
+  (* ignore spacing and newline characters *)
+  [' ' '\009' '\012' '\n']+     { main lexbuf }
+| "("   { Parser.LPAREN }
+| ")"   { Parser.RPAREN }
+| ";"   { Parser.SEMI }
+| "\."   { Parser.ABS }
+| "Ap"   { Parser.APP }
+| ['0'-'9'] {Parser.VAR (int_of_string (Lexing.lexeme lexbuf))}
+| eof   { exit 0 }
+| _     { raise (Error (Printf.sprintf "At offset %d: unexpected character." (Lexing.lexeme_start lexbuf))) }
+
