untype_lambda/ocaml/chap6/src/parser.mly
@@ -1,0 +1,33 @@
+%{
+  open Eval
+
+  let rec change n =
+    match n with
+    | 0 -> O
+    | _ -> S (change (n - 1))
+%}
+
+
+%token LPAREN RPAREN SEMI
+%token APP
+%token ABS 
+%token <int> VAR
+
+%start toplevel
+%type <Eval.term> toplevel
+%%
+
+toplevel :
+  e=Expr SEMI {e}
+
+Expr :
+  APP t1=Expr t2=Expr  {App (t1, t2)}
+  | e=AExpr {e}
+
+AExpr :
+  ABS e=Expr {Abs e}
+  | e=VExpr {e}
+
+VExpr :
+  n = VAR  {Var (change n)}
+  | LPAREN e=Expr RPAREN {e}
