untype_lambda/ocaml/chap6/src/print.ml
@@ -1,0 +1,17 @@
+open Eval
+
+let rec nat2int n = 
+  match n with
+  | O    -> 0
+  | S n' -> 1 + (nat2int n')
+
+let rec eval_string t =
+  match t with
+  | App (t1, t2) -> "App ( " ^ (eval_string t1) ^ " ) ( " ^ (eval_string t2) ^ " )"
+  | Abs t1       -> "Abs ( " ^ (eval_string t1) ^ " )"
+  | Var n        -> string_of_int (nat2int n)
+
+let eval t =
+  match step t with
+  | Some t' -> t'
+  | None    -> t
