untype_lambda/chap6.v
@@ -1,3 +1,6 @@
+Require Coq.extraction.Extraction.
+Extraction Language OCaml.
+
 Inductive term : Type :=
 | Var : nat -> term
 | Abs : term -> term
@@ -46,15 +49,112 @@ Notation "'[' x ':=' s ']' t" := (subst x s t) (at level 20).
 
 Inductive eval : term -> term -> Prop :=
   | E_App1 : forall t1 t1' t2,
-         t1 --> t1' ->
-         App t1 t2 --> App t1' t2
+      t1 --> t1' ->
+      App t1 t2 --> App t1' t2
   | E_App2 : forall v1 t2 t2',
-         value v1 ->
-         t2 --> t2' ->
-         App v1 t2 --> App v1 t2'
+      value v1 ->
+      t2 --> t2' ->
+      App v1 t2 --> App v1 t2'
   | E_AppAbs : forall t1 v2,
-         value v2 ->
-         App (Abs t1) v2 -->
-             up beta_ShiftNum ([0 := up 1 (v2)] t1)
+      value v2 ->
+      App (Abs t1) v2 -->
+          up beta_ShiftNum ([0 := up 1 (v2)] t1)
 
   where " t '-->' t' " := (eval t t').
+
+Definition relation (X : Type) := X -> X -> Prop.
+
+Inductive multi {X : Type} (R : relation X) : relation X :=
+  | multi_refl : forall (x : X), multi R x x
+  | multi_step : forall (x y z : X),
+                    R x y ->
+                    multi R y z ->
+                    multi R x z.
+
+Notation multieval := (multi eval).
+Notation "t1 '-->*' t2" := (multieval t1 t2) (at level 40).
+
+Definition vb (t: term) :=
+  match t with
+  | Abs _ => true
+  | _ => false
+  end.
+
+Lemma vbValue : forall t,
+    vb t = true <-> value t.
+Proof.
+  destruct t; split; intros; inversion H; auto.
+  apply v_abs.
+Qed.
+
+Inductive optiont : Type :=
+| Some (t: term)
+| None.
+
+Fixpoint step (t: term) : optiont :=
+  match t with
+  | App t1 t2 =>
+    match t1 with
+    | Abs t3 =>
+      if vb t2 then
+        Some (up beta_ShiftNum ([0 := up 1 (t2)] t3)) else
+        match step t2 with
+        | Some t2' => Some (App t1 t2')
+        | None => None
+        end
+    | _ =>
+      match step t1 with
+      | Some t1' =>
+        Some (App t1' t2)
+      | None => None
+      end
+    end
+  | _ => None
+  end.
+Extraction "ocaml/chap6/src/eval.ml" step.
+
+Lemma stepeval : forall t t',
+    t --> t' <-> step t = Some t'.
+Proof.
+  split; intros.
+  -
+    induction H.
+    +
+      simpl. destruct t1. inversion H. inversion H.
+      rewrite IHeval. reflexivity.
+    +
+      simpl. inversion H; subst. destruct t2. inversion H0. inversion H0. rewrite IHeval. simpl. reflexivity.
+    +
+      inversion H; subst. simpl. reflexivity.
+  -
+    generalize dependent t'.
+    induction t; intros. inversion H. inversion H.
+    simpl in H.
+    destruct t1. inversion H. destruct (vb t2) eqn:IH2. inversion H. apply E_AppAbs. apply vbValue; auto.
+    destruct (step t2) eqn:IHH. inversion H.
+    apply E_App2. apply v_abs. apply IHt2. reflexivity.
+    inversion H.
+    destruct (step (App t1_1 t1_2)). inversion H. apply E_App1. apply IHt1. reflexivity.
+    inversion H.
+Qed.
+
+
+(*評価の一意性*)
+Lemma determine : forall t t' t'',
+    t --> t' -> t --> t'' -> t' = t''.
+Proof.
+  intros; generalize dependent t''. induction H; intros.
+  -
+    inversion H0; subst.
+    apply IHeval in H4. rewrite H4; reflexivity.
+    inversion H3; subst. inversion H.
+    inversion H.
+  -
+    inversion H1; subst. inversion H; subst; inversion H5.
+    apply IHeval in H6. rewrite H6; reflexivity.
+    inversion H5; subst; inversion H0.
+  -
+    inversion H; inversion H0; subst.
+    inversion H5. inversion H6.
+    reflexivity.
+Qed.
